reals/fast/CRarctan_small.v
@@ -40,12 +40,12 @@ Opaque inj_Q CR.
 Section ArcTanSeries.
 Variable a:Q.
 
-Definition arcTanSequence := (mult_Streams (everyOther recip_positives) (powers_help (a^2) a)).
+Definition arctanSequence := (mult_Streams (everyOther recip_positives) (powers_help (a^2) a)).
 
-Lemma Str_nth_arcTanSequence : forall n, (Str_nth n arcTanSequence == (1#P_of_succ_nat (2*n))*a^(1+2*n)%nat)%Q.
+Lemma Str_nth_arctanSequence : forall n, (Str_nth n arctanSequence == (1#P_of_succ_nat (2*n))*a^(1+2*n)%nat)%Q.
 Proof.
 intros n.
-unfold arcTanSequence.
+unfold arctanSequence.
 unfold mult_Streams.
 rewrite Str_nth_zipWith.
 rewrite Str_nth_everyOther.
@@ -78,7 +78,7 @@ apply Qle_trans with 0.
 assumption.
 Qed.
 
-Lemma arcTanSequence_dnn : DecreasingNonNegative arcTanSequence.
+Lemma arctanSequence_dnn : DecreasingNonNegative arctanSequence.
 Proof.
 rapply mult_Streams_dnn.
  apply everyOther_dnn.
@@ -88,9 +88,9 @@ apply powers_help_dnn.
 destruct Ha; assumption.
 Qed.
 
-Lemma arcTanSequence_zl : Limit arcTanSequence 0.
+Lemma arctanSequence_zl : Limit arctanSequence 0.
 Proof.
-unfold arcTanSequence.
+unfold arctanSequence.
 apply mult_Streams_zl with (1#1)%Qpos.
  apply everyOther_zl.
  apply recip_positives_zl.
@@ -100,14 +100,14 @@ Defined.
 
 End ArcTanSeries.
 
-Definition rational_arcTan_small_pos (a:Q) (p: 0 <= a <= 1) : CR := 
- InfiniteAlternatingSum (arcTanSequence_dnn p) (arcTanSequence_zl p).
+Definition rational_arctan_small_pos (a:Q) (p: 0 <= a <= 1) : CR := 
+ InfiniteAlternatingSum (arctanSequence_dnn p) (arctanSequence_zl p).
 
-Lemma rational_arcTan_small_pos_correct : forall (a:Q) Ha, a < 1 ->
- (@rational_arcTan_small_pos a Ha == IRasCR (ArcTan (inj_Q IR a)))%CR.
+Lemma rational_arctan_small_pos_correct : forall (a:Q) Ha, a < 1 ->
+ (@rational_arctan_small_pos a Ha == IRasCR (ArcTan (inj_Q IR a)))%CR.
 Proof.
 intros a Ha Ha0.
-unfold rational_arcTan_small_pos.
+unfold rational_arctan_small_pos.
 rewrite InfiniteAlternatingSum_correct'.
 apply IRasCR_wd.
 assert (X:(olor ([--]One) One (inj_Q IR a))).
@@ -127,7 +127,7 @@ eapply eq_transitive_unfolded;
  [|apply (arctan_series (inj_Q IR a) (arctan_series_convergent_IR) X)].
 rapply series_sum_wd.
 intros n.
-change (inj_Q IR ((- (1)) ^ n * Str_nth n (arcTanSequence a))[=]
+change (inj_Q IR ((- (1)) ^ n * Str_nth n (arctanSequence a))[=]
 (([--]One[^]n[/]nring (R:=IR) (S (2 * n))[//]nringS_ap_zero IR (2 * n))[*]
  (inj_Q IR a)[^](2 * n + 1))).
 rstepr (([--]One[^]n)[*]((inj_Q IR a)[^](2*n+1)[/]nring (R:=IR) (S (2 * n))[//]nringS_ap_zero IR (2 * n))).
@@ -146,14 +146,14 @@ apply mult_cancel_lft with (nring (R:=IR) (S (2 * n))).
  apply nringS_ap_zero.
 rstepr (inj_Q IR a[^](2 * n + 1)).
 stepr (inj_Q IR (a^(2*n+1)%nat)) by apply inj_Q_power.
-stepl ((inj_Q IR (nring (S (2*n))))[*]inj_Q IR (Str_nth n (arcTanSequence a))) by
+stepl ((inj_Q IR (nring (S (2*n))))[*]inj_Q IR (Str_nth n (arctanSequence a))) by
  apply mult_wdl; apply inj_Q_nring.
-stepl (inj_Q IR (nring (S (2*n))[*]Str_nth n (arcTanSequence a)))
+stepl (inj_Q IR (nring (S (2*n))[*]Str_nth n (arctanSequence a)))
  by apply inj_Q_mult.
 apply inj_Q_wd.
 csetoid_rewrite (nring_Q (S (2*n))).
-change (S (2 * n)*Str_nth n (arcTanSequence a)==a ^ (2 * n + 1)%nat).
-rewrite Str_nth_arcTanSequence.
+change (S (2 * n)*Str_nth n (arctanSequence a)==a ^ (2 * n + 1)%nat).
+rewrite Str_nth_arctanSequence.
 rewrite (Qmake_Qdiv).
 rewrite plus_comm.
 generalize (a^(2*n+1)%nat).
@@ -166,10 +166,10 @@ rewrite <- POS_anti_convert.
 auto with *.
 Qed.
 
-Definition rational_arcTan_small (a:Q) (p: -(1) <= a <= 1) : CR.
+Definition rational_arctan_small (a:Q) (p: -(1) <= a <= 1) : CR.
 intros a.
 destruct (Qle_total a 0); intros Ha.
- refine (-(@rational_arcTan_small_pos (-a)%Q _))%CR.
+ refine (-(@rational_arctan_small_pos (-a)%Q _))%CR.
  abstract (
  split;
  [(replace RHS with (0+-a) by ring);
@@ -179,19 +179,19 @@ destruct (Qle_total a 0); intros Ha.
   (replace RHS with (a + - - (1)) by ring);
   rewrite <- Qle_minus_iff;
   destruct Ha; assumption]).
-apply (@rational_arcTan_small_pos a).
+apply (@rational_arctan_small_pos a).
 abstract (
 split;[|destruct Ha; assumption];
  apply Qnot_lt_le; apply Qle_not_lt; assumption).
 Defined.
 
-Lemma rational_arcTan_small_correct : forall (a:Q) Ha, -(1) < a -> a < 1 ->
- (@rational_arcTan_small a Ha == IRasCR (ArcTan (inj_Q IR a)))%CR.
+Lemma rational_arctan_small_correct : forall (a:Q) Ha, -(1) < a -> a < 1 ->
+ (@rational_arctan_small a Ha == IRasCR (ArcTan (inj_Q IR a)))%CR.
 Proof.
 intros a Ha Ha0 Ha1.
-unfold rational_arcTan_small.
+unfold rational_arctan_small.
 destruct (Qle_total a 0);
- rewrite rational_arcTan_small_pos_correct.
+ rewrite rational_arctan_small_pos_correct.
    rewrite Qlt_minus_iff.
    replace RHS with (a + - - (1)) by ring.
    rewrite <- Qlt_minus_iff.
